CODIGO/GRAFOS/Transformations/IndependentSetToVertexCover.dfy
@@ -3,34 +3,58 @@ include "../Problems/IndependentSet.dfy"
 include "../Problems/VertexCover.dfy"
 
 function IndependentSet_to_VertexCover(graph:Graph, k:int) : (r:(Graph,int))
+    requires isValidGraph(graph)
 {
     (graph,|graph.0|-k)
 }
 
 lemma IndependentSet_VertexCover(graph:Graph, k:int)
-  ensures var (Vgraph,Vk):= IndependentSet_to_VertexCover(graph,k);
-          IndependentSet(graph,k) <==> IndependentSet(Vgraph,Vk)
+    requires isValidGraph(graph)
+    ensures var (Vgraph,Vk):= IndependentSet_to_VertexCover(graph,k);
+        IndependentSet(graph,k) <==> VertexCover(Vgraph,Vk)
 { 
     IndependentSet_VertexCover1(graph,k);
     IndependentSet_VertexCover2(graph,k);
 }
 
+lemma aux (IndepSet:set<Node>, vCover:set<Node>, graph:Graph)
+    requires IndepSet + vCover == graph.0
+    requires IndepSet * vCover == {}
+    ensures forall e | e in graph.1 :: |IndepSet * e| + |vCover * e| == |e|
+
+
 lemma IndependentSet_VertexCover1(graph:Graph, k:int)
+    requires isValidGraph(graph)
     ensures var (Vgraph,Vk) := IndependentSet_to_VertexCover(graph,k);
           IndependentSet(graph,k) <== VertexCover(Vgraph,Vk)
 {   
     var (Vgraph,Vk) := IndependentSet_to_VertexCover(graph,k);
     if (VertexCover(Vgraph,Vk)) {
-        asdfasdfsadf
+        var vCover:set<Node> :| isVertexCover(vCover,Vgraph.1) && |vCover| <= Vk && vCover <= Vgraph.0;
+
+        var IndepSet:set<Node> := graph.0 - vCover;
+
+        // Demostracion 1 : isIndependentSet(IndepSet,graph.1)
+        aux (IndepSet, vCover, graph); // Por cada arista, hay uno o dos elementos de vertexCover, lo que significa que debe haber uno de IndepSet        
+        
+        assert isIndependentSet(IndepSet,graph.1) && |IndepSet| >= k && IndepSet <= graph.0;
     }
 }
 
 lemma IndependentSet_VertexCover2(graph:Graph, k:int)
+    requires isValidGraph(graph)
     ensures var (Vgraph,Vk) := IndependentSet_to_VertexCover(graph,k);
           IndependentSet(graph,k) ==> VertexCover(Vgraph,Vk)
 {
-
     if (IndependentSet(graph,k)) {
-        
+        var (Vgraph,Vk) := IndependentSet_to_VertexCover(graph,k);
+        var IndepSet:set<Node> :| isIndependentSet(IndepSet,graph.1) && |IndepSet| >= k && IndepSet <= graph.0;
+
+        var vCover:set<Node> := graph.0 - IndepSet;
+
+        // Demostracion 1 : isVertexCover(vCover,graph.1)
+        aux(IndepSet, vCover, graph); 
+
+        assert isVertexCover(vCover,Vgraph.1) && |vCover| <= Vk && vCover <= Vgraph.0;
     }
 }
