CODIGO/GRAFOS/Transformations/VertexCoverToIndependentSet.dfy
@@ -1,0 +1,60 @@
+include "../Auxiliar/Graph.dfy"
+include "../Problems/VertexCover.dfy"
+include "../Problems/IndependentSet.dfy"
+
+function VertexCover_to_IndependentSet(graph:Graph, k:int) : (r:(Graph,int))
+    requires isValidGraph(graph)
+{
+    (graph,|graph.0|-k)
+}
+
+lemma VertexCover_IndependentSet(graph:Graph, k:int)
+    requires isValidGraph(graph)
+    ensures var (Vgraph,Vk):= VertexCover_to_IndependentSet(graph,k);
+        VertexCover(graph,k) <==> IndependentSet(Vgraph,Vk)
+{ 
+    VertexCover_IndependentSet1(graph,k);
+    VertexCover_IndependentSet2(graph,k);
+}
+
+lemma aux (IndepSet:set<Node>, vCover:set<Node>, graph:Graph)
+    requires IndepSet + vCover == graph.0
+    requires IndepSet * vCover == {}
+    ensures forall e | e in graph.1 :: |IndepSet * e| + |vCover * e| == |e|
+
+
+lemma VertexCover_IndependentSet1(graph:Graph, k:int)
+    requires isValidGraph(graph)
+    ensures var (Vgraph,Vk) := VertexCover_to_IndependentSet(graph,k);
+          VertexCover(graph,k) <== IndependentSet(Vgraph,Vk)
+{   
+    var (Vgraph,Vk) := VertexCover_to_IndependentSet(graph,k);
+    if (IndependentSet(Vgraph,Vk)) {
+        var IndepSet:set<Node> :| isIndependentSet(IndepSet,Vgraph.1) && |IndepSet| >= Vk && IndepSet <= Vgraph.0;
+
+        var vCover:set<Node> := graph.0 - IndepSet;
+
+        // Demostracion 1 : isVertexCover(IndepSet,graph.1)
+        aux (IndepSet, vCover, graph); // Por cada arista, hay uno o dos elementos de IndependentSet, lo que significa que debe haber uno de IndepSet        
+        
+        assert isVertexCover(vCover,graph.1) && |vCover| <= k && vCover <= graph.0;
+    }
+}
+
+lemma VertexCover_IndependentSet2(graph:Graph, k:int)
+    requires isValidGraph(graph)
+    ensures var (Vgraph,Vk) := VertexCover_to_IndependentSet(graph,k);
+          VertexCover(graph,k) ==> IndependentSet(Vgraph,Vk)
+{
+    if (VertexCover(graph,k)) {
+        var (Vgraph,Vk) := VertexCover_to_IndependentSet(graph,k);
+        var vCover:set<Node> :| isVertexCover(vCover,graph.1) && |vCover| <= k && vCover <= graph.0;
+
+        var IndepSet:set<Node> := graph.0 - vCover;
+
+        // Demostracion 1 : isIndependentSet(vCover,graph.1)
+        aux(IndepSet, vCover, graph); 
+
+        assert isIndependentSet(IndepSet,Vgraph.1) && |IndepSet| >= Vk && vCover <= Vgraph.0;
+    }
+}
